proof/invariant-abstract/ARM_HYP/ArchDeterministic_AI.thy
@@ -16,7 +16,8 @@ context Arch begin global_naming ARM
 
 named_theorems Deterministic_AI_assms
 
-crunch valid_list[wp, Deterministic_AI_assms]: vcpu_save, vcpu_enable, vcpu_disable, vcpu_restore valid_list
+crunch valid_list[wp, Deterministic_AI_assms]:
+ vcpu_save, vcpu_enable, vcpu_disable, vcpu_restore, arch_tcb_set_ipc_buffer valid_list
   (wp: crunch_wps simp: unless_def crunch_simps)
 
 lemma vcpu_switch_valid_list[wp, Deterministic_AI_assms]:
