proof/invariant-abstract/ARM_HYP/ArchUntyped_AI.thy
@@ -308,7 +308,7 @@ lemma delete_objects_rewrite[Untyped_AI_assms]:
     od"
   apply (clarsimp simp:delete_objects_def freeMemory_def word_size_def)
   apply (subgoal_tac "is_aligned (ptr &&~~ mask sz) sz")
-  apply (subst mapM_storeWord_clear_um)
+  apply (subst mapM_storeWord_clear_um[simplified word_size_def word_size_bits_def])
   apply (simp)
   apply simp
   apply (simp add:range_cover_def)
@@ -321,7 +321,7 @@ declare store_pde_pred_tcb_at [wp]
 
 (* nonempty_table *)
 definition
-  nonempty_table :: "word32 set \<Rightarrow> Structures_A.kernel_object \<Rightarrow> bool"
+  nonempty_table :: "machine_word set \<Rightarrow> Structures_A.kernel_object \<Rightarrow> bool"
 where
  "nonempty_table S ko \<equiv>
     (a_type ko = AArch APageTable \<or> a_type ko = AArch APageDirectory)
