proof/invariant-abstract/Untyped_AI.thy
@@ -20,7 +20,7 @@ context begin interpretation Arch .
 requalify_consts
   region_in_kernel_window
   arch_default_cap
-  second_level_tables
+(*  second_level_tables *) (* not used in ARMHYP *)
 end
 
 primrec
