spec/abstract/ARM_HYP/ArchCSpace_A.thy
@@ -20,6 +20,25 @@ imports
 begin
 context Arch begin global_naming ARM_A
 
+definition cnode_guard_size_bits :: "nat"
+where
+  cnode_guard_size_bits_def [simp]: "cnode_guard_size_bits \<equiv> 5"
+
+definition cnode_padding_bits :: "nat"
+where
+  cnode_padding_bits_def [simp]: "cnode_padding_bits \<equiv> 3"
+
+text {* On a user request to modify a cnode capability, extract new guard bits and guard. *}
+definition
+  update_cnode_cap_data :: "data \<Rightarrow> nat \<times> data" where
+ "update_cnode_cap_data w \<equiv>
+    let
+      guard_bits = 18;
+      guard_size' = unat ((w >> cnode_padding_bits) && mask cnode_guard_size_bits);
+      guard'' = (w >> (cnode_padding_bits + cnode_guard_size_bits)) && mask guard_bits
+    in (guard_size', guard'')"
+
+
 text {* For some purposes capabilities to physical objects are treated
 differently to others. *}
 definition
