spec/abstract/ARM_HYP/ArchTcb_A.thy
@@ -1,0 +1,29 @@
+(*
+ * Copyright 2014, General Dynamics C4 Systems
+ *
+ * This software may be distributed and modified according to the terms of
+ * the GNU General Public License version 2. Note that NO WARRANTY is provided.
+ * See "LICENSE_GPLv2.txt" for details.
+ *
+ * @TAG(GD_GPL)
+ *)
+
+(*
+Arch-specific functions for the abstract model of CSpace.
+*)
+
+chapter "Architecture-specific TCB functions"
+
+theory ArchTcb_A
+imports "../KHeap_A"
+begin
+
+context Arch begin global_naming ARM_A
+
+definition
+  arch_tcb_set_ipc_buffer :: "machine_word \<Rightarrow> vspace_ref \<Rightarrow> (unit, 'a::state_ext) s_monad"
+where
+  "arch_tcb_set_ipc_buffer target ptr \<equiv> as_user target $ set_register TPIDRURW ptr"
+
+end
+end
