spec/abstract/ARM_HYP/Arch_Structs_A.thy
@@ -360,6 +360,10 @@ where
          | ASIDPool f               \<Rightarrow> AASIDPool
          | VCPU v                   \<Rightarrow> AVCPU)"
 
+text {* For implementation reasons the badge word has differing amounts of bits *}
+definition
+  badge_bits :: nat where
+  badge_bits_def [simp]: "badge_bits \<equiv> 28"
 end
 
 section "Arch-specific tcb"
